Multiple and Submultiple Angles
********************************
Multiple Angles
===============
An angle of the form :math:`nA,` where :math:`n` is an integer is called a *multiple angle.* For example, :math:`2A, 3A, 4A,
\ldots` are multiple angles of :math:`A.`

Trigonometrical Ratios of :math:`2A`
------------------------------------
From previous chapter we know that :math:`\sin(A + B) = \sin A\cos B + \cos A\sin B`

Substituting :math:`B = A,` we get

:math:`\sin 2A = 2\sin A\cos A`

Similarly, :math:`\cos 2A = \cos^2A - \sin^2A = 2\cos^2A -  1 = 1 - 2\sin^2A` (recall formula from previous chapter and substitute
:math:`B = A` :math:`\cos^2A = 1 -\sin^2A` and :math:`\sin^2A = 1 - \cos^2a`)

Also, :math:`\tan 2A = \frac{2\tan A}{1 - \tan^2A}` (recall formula from previous chapter and put :math:`B = A`)

:math:`\sin 2A` and :math:`\cos 2A` in terms of :math:`\tan A`
--------------------------------------------------------------
:math:`\sin 2A = \frac{2\sin A\cos A}{\sin^2A + \cos^2A}[\because \sin^2A + \cos^2A = 1]`

Dividing both numerator and denominator by :math:`\cos^2A,` we get

:math:`\sin 2A = \frac{2\tan A}{1 + \tan^2A}`

:math:`\cos A = \cos^2A - \sin^2A = \frac{\cos^2A - \sin^2A}{\cos^2A + \sin^2A}[\because \sin^2A + \cos^2A = 1]`

Dividing both numerator and denominator by :math:`\cos^2A,` we get

:math:`\cos 2A = \frac{1 - \tan^2A}{1 + \tan^2A} = \frac{\cot^2A - 1}{\cot^2A + 1}`

Trigonometrical Ratios of :math:`3A`
------------------------------------
:math:`\sin 3A = \sin2A\cos A + \cos 2A\sin A = 2\sin A\cos^2 A + \cos^2A\sin A - \sin^3A`

:math:`= 2\sin A(1 - \sin^2A) + (1 - 2\sin^2A)\sin A - \sin^3A`

:math:`= 3\sin A - 4\sin^3A`

:math:`\cos 3A = \cos2A\cos A - \sin 2A\sin A = (2\cos^2A - 1)\cos A - 2\sin^2 A\cos A`

:math:`= 2\cos^3A - \cos A - 2(1 - \cos^2A)\cos A`

:math:`= 4\cos^3 A - 3\cos A`

We know that :math:`\tan(A + B + C) = \frac{\tan A + \tan B + \tan C - \tan A\tan B\tan C}{1 - \tan A\tan B - \tan B\tan C - \tan
C\tan A}`

Putting :math:`B = A` and :math:`C = A,` we get

:math:`\tan 3A = \frac{3\tan A - \tan^3A}{1 - 3\tan^2A}`

Similarly :math:`\cot 3A = \frac{\cot^3 A - 3\cot A}{3\cot^2A - 1}`

Some Important Formulae
-----------------------
1. :math:`\cos2A = 1 - 2\sin^2A \Rightarrow \sin^2A = \frac{1}{2}(1 - \cos2A)`

2. :math:`\cos2A = 2\cos^2 - 1 \Rightarrow \cos^2A = \frac{1}{2}(1 + \cos2A)`

3. :math:`\sin 3A = 3\sin A - 4\sin^3A \Rightarrow sin^3A = \frac{1}{2}(3\sin A - \sin3A)`

4. :math:`\cos 3A = 4\cos^3A - 3\cos A \Rightarrow \cos^3A = \frac{1}{4}(\cos3A + 3\cos A)`

Submultiple Angles
==================
An angle of the form :math:`\frac{A}{n},` where :math:`n` is an integer is called a *submultiple angle.* For exmaple,
:math:`\frac{A}{2}, \frac{A}{3}, \frac{A}{4}, \ldots` are submultiple angles of :math:`A.`

Trigonometrical Ratios of :math:`A/2`
-------------------------------------
We know that, :math:`\sin 2A = 2\sin A\cos A.` Putting :math:`A=A/2,` we get

:math:`\sin A = 2\sin A/2\cos A/2`

:math:`\cos 2A = \cos^2A - \sin^A.` Putting :math:`A = A/2,` we get

:math:`\cos A - \cos^2\frac{A}{2} - \sin^2\frac{A}{2}`

:math:`\cos 2A = 2\cos^2A - 1.` Putting :math:`A = A/2,` we get

:math:`\cos A = 2\cos^2\frac{A}{2} - 1`

:math:`\cos 2A = 1 - 2\sin^2A.` Putting :math:`A = A/2,` we get

:math:`\cos A = 1 - 2\sin^2\frac{A}{2}`

:math:`\tan 2A = \frac{2\tan A}{1 - \tan^2A}.` Putting :math:`A = A/2,` we get

:math:`\tan A = \frac{2\tan \frac{A}{2}}{1 - \tan^2\frac{A}{2}}`

:math:`\sin 2A = \frac{2\tan A}{1 + \tan^2A} \therefore \sin A = \frac{2\tan \frac{A}{2}}{1 + \tan^2\frac{A}{2}}`

:math:`\cos 2A = \frac{1 - \tan^2A}{1 + \tan^2A} \therefore \cos A = \frac{1 - \tan^2\frac{A}{2}}{1 + \tan^2\frac{A}{2}}`

:math:`\cot 2A = \frac{\cot^2A - 1}{2\cot A} \therefore \cot A = \frac{\cot^2\frac{A}{2} - 1}{2\cot \frac{A}{2}}`

Trigonometrical Ratios of :math:`A/3`
-------------------------------------
:math:`\sin 3A = 3\sin A - 4\sin^3A.` Putting :math:`A = \frac{A}{3},` we get

:math:`\sin A = \frac{3}{\sin \frac{A}{3}} - 4\sin^3\frac{A}{3}`

:math:`\cos 3A = 4\cos^3A - 3\cos A`. Putting :math:`A = \frac{A}{3},` we get

:math:`\cos A = 4\cos^3\frac{A}{3} - 3\cos \frac{A}{3}`

:math:`\tan 3A = \frac{3\tan A - \tan^3A}{1 - 3\tan^2A}`

:math:`\tan A = \frac{3\tan\frac{A}{3} - \tan^3\frac{A}{3}}{1 - 3\tan^2\frac{A}{3}}`

Values of :math:`cos A/2, \sin A/2` and :math:`\tan A/2` in terms of :math:`\cos A`
-----------------------------------------------------------------------------------
:math:`\cos^2\frac{A}{2} = \frac{1 + \cos A}{2} \therefore \cos \frac{A}{2} = \sqrt{\frac{1 + \cos A}{2}}`

:math:`\sin^2\frac{A}{2} = \frac{1 - \cos A}{}2 \therefore \sin \frac{A}{2} = \sqrt{\frac{1 - \cos A}{2}}`

:math:`\tan^2\frac{A}{2} = \frac{1 - \cos A}{1 + \cos A} \therefore \tan\frac{A}{2} = \sqrt{\frac{1 - \cos A}{1 + \cos A}}`

Values of :math:`\sin A/2` and :math:`\cos A/2` in terms of :math:`\sin A`
--------------------------------------------------------------------------
:math:`\left(\cos \frac{A}{2} + \sin\frac{A}{2}\right)^2 = \cos^2\frac{A}{2} + \sin^2\frac{A}{2} + 2\cos\frac{A}{2}\sin\frac{A}{2}`

:math:`= 1 + \sin A \Rightarrow \cos \frac{A}{2} + \sin \frac{A}{2} = \sqrt{1 + \sin A}`

Similarly, :math:`\cos \frac{A}{2} - \sin \frac{A}{2} = \sqrt{1 - \sin A}`

Adding, we get :math:`\cos \frac{A}{2} = \pm\frac{1}{2}\sqrt{1 + \sin A} \pm\frac{1}{2}\sqrt{1 - \sin A}`

Subtracting, we get :math:`\cos \frac{A}{2} = \pm\frac{1}{2}\sqrt{1 + \sin A} \mp\frac{1}{2}\sqrt{1 - \sin A}`

Value of :math:`\sin 18^\circ` and :math:`\cos 72^\circ`
--------------------------------------------------------
Let :math:`A = 18^\circ,` then :math:`\sin 5A = 90^\circ \therefore 2A + 3A = 90^\circ`

:math:`\sin2A = \sin(90^\circ - \sin 3A) \therefore 2\sin A\cos A = 4\cos^3A - 3\cos A`

Dividing both sides by :math:`\cos A,` we get

:math:`2\sin A = 4\cos^2A - 3 = 4(1 - \sin^2A) - 3`

:math:`4\sin^2A + 2\sin A - 1 = 0`

:math:`\sin A = \frac{-1\pm\sqrt{5}}{4}`

However, since :math:`A= 18^\circ\therefore \sin A > 0`

:math:`\therefore \sin18^\circ = \frac{-1 + \sqrt{5}}{4}`

:math:`\therefore \sin(90^\circ - 18^\circ) = \cos72^\circ = \frac{\sqrt{5} - 1}{4}`

Value of :math:`\cos 18^\circ` and :math:`\sin 72^\circ`
--------------------------------------------------------
:math:`\cos^218^\circ = 1 - \sin^218^\circ = 1 - \left(\frac{\sqrt{5} - 1}{4}\right)^2`

:math:`= \frac{10 + 2\sqrt{5}}{16}\therefore \cos18^\circ = \frac{1}{4}\sqrt{10 + 2\sqrt{5}}[\because \cos18^\circ > 0]`

:math:`\cos(90^\circ - 18^\circ) = \sin72^\circ = \frac{1}{4}\sqrt{10 + 2\sqrt{5}}`

Value of :math:`\tan 18^\circ` and :math:`\tan 72^\circ`
--------------------------------------------------------
:math:`\tan 18^\circ = \frac{\sin18^\circ}{\cos18^\circ} = \frac{\sqrt{5} - 1}{\sqrt{10 + 2\sqrt{5}}}`

:math:`\tan18^\circ\cot18^\circ = 1\Rightarrow \tan72^\circ = \frac{1}{\tan18^\circ} = \frac{\sqrt{10 + 2\sqrt{5}}}{\sqrt{5} - 1}`

Value of :math:`\cos 36^\circ` and :math:`\sin 54^\circ`
--------------------------------------------------------
:math:`\cos 36^\circ = 1 - 2\sin^218^\circ = 1 - 2\left(\frac{\sqrt{5} - 1}{4}\right)^2`

:math:`= \frac{\sqrt{5} + 1}{4}`

:math:`\sin 54^\circ = \sin(90^\circ - 36^\circ) = \cos36^\circ = \frac{\sqrt{5} + 1}{4}`

Value of :math:`\sin 36^\circ` and :math:`\cos 54^\circ`
--------------------------------------------------------
:math:`\sin36^\circ = 1 - \cos^236^\circ = 1 - \left(\frac{\sqrt{5} + 1}{4}\right)^2`

:math:`= \frac{1}{4}\sqrt{10 - 2\sqrt{5}}`

:math:`\cos54^\circ = \cos(90^\circ - 36^\circ) = \sin36^\circ = \frac{1}{4}\sqrt{10 - 2\sqrt{5}}`

Several other angles like, :math:`9^\circ, 15^\circ, 22\frac{1}{2}^\circ, 7\frac{1}{2}^\circ` etc can be found similarrly.

Problems
========
1. Find the value of :math:`\sin 2A,` when

   i) :math:`\cos A = \frac{3}{5}`

   ii) :math:`\sin A = \frac{12}{13}`

   iii) :math:`\tan A = \frac{16}{63}`

2. Find the value of :math:`\cos 2A,` when

   i. :math:`\cos A = \frac{15}{17}`

   ii. :math:`\sin A = \frac{4}{5}`

   iii. :math:`\tan A = \frac{5}{12}`

3. If :math:`\tan A = \frac{b}{a},` find the value of :math:`a\cos 2A+ b\sin 2A`

Prove that

4. :math:`\frac{\sin 2A}{1 + \cos 2A} = \tan A`

5. :math:`\frac{\sin 2A}{1 - \cos 2A} = \cot A`

6. :math:`\frac{1 - \cos 2A}{1 + \cos 2A} = \tan^2A`

7. :math:`\tan A + \cot A = 2\cosec 2A`

8. :math:`\tan A - \cot A = -2\cot2A`

9. :math:`\cosec 2A + \cot 2A = \cot A`

10. :math:`\frac{1 - \cos A + \cos B - \cos(A + B)}{1 + \cos A - \cos B - \cos(A + B)} = \tan\frac{A}{2}\cot\frac{B}{2}`

11. :math:`\frac{\cos A}{1 \mp \sin A} = \tan\left(45^\circ \pm \frac{A}{2}\right)`

12. :math:`\frac{\sec 8A - 1}{\sec 4A - 1} = \frac{\tan 8A}{\tan 2A}`

13. :math:`\frac{1 + \tan^2(45^\circ - A)}{1 - \tan^2(45^\circ - A)} = \cosec 2A`

14. :math:`\frac{\sin A + \sin B}{\sin A - \sin B} = \frac{\tan \frac{A + B}{2}}{\tan \frac{A - B}{2}}`

15. :math:`\frac{\sin^2A - \sin^2B}{\sin A\cos A - \sin B\cos B} = \tan(A + B)`

16. :math:`\tan\left(\frac{\pi}{4} + A\right) - \tan\left(\frac{\pi}{4} - A\right) = 2\tan 2A`

17. :math:`\frac{\cos A + \sin A}{\cos A - \sin A} - \frac{\cos A - \sin A}{\cos A + \sin A} = 2\tan 2A`

18. :math:`\cot (A + 15^\circ) - \tan(A - 15^\circ) = \frac{4\cos 2A}{1 + 2\sin 2A}`

19. :math:`\frac{\sin A + \sin2A}{1 + \cos A + \cos 2A} = \tan A`

20. :math:`\frac{1 + \sin A - \cos A }{1 + \sin A + cos A} = \tan \frac{A}{2}`

21. :math:`\frac{\sin(n + 1)A - \sin(n - 1)A}{\cos(n + 1)A + 2\cos nA + \cos(n - 1)A} = \tan \frac{A}{2}`

22. :math:`\frac{\sin(n + 1)A + 2\sin nA + \sin(n - 1)A}{\cos(n - 1) - \cos(n + 1)A} = \cot \frac{A}{2}`

23. :math:`\sin(2n + 1)A\sin A = \sin^2(n + 1)A - \sin^2nA`

24. :math:`\frac{\sin(A + 3B) + \sin(3A + B)}{\sin 2A + \sin 2B} = 2\cos(A + B)`

25. :math:`\sin 3A + \sin 2A - \sin A = 4\sin A\cos \frac{A}{2}\cos \frac{3A}{2}`

26. :math:`\tan 2A = (\sec 2A + 1)\sqrt{\sec^2A - 1}`

27. :math:`\cos^32A + 3\cos 2A = 4(\cos^6A - \sin^6A)`

28. :math:`1 + \cos^22A = 2(\cos^4A + \sin^4A)`

29. :math:`\sec^2A(1 + \sec2A) = 2\sec2A`

30. :math:`\cosec A - 2\cot 2A\cos A = 2\sin A`

31. :math:`\cot A = \frac{1}{2}\left(\cot\frac{A}{2} - \tan\frac{A}{2}\right)`

32. :math:`\sin A\sin(60^\circ - A)\sin(60^\circ + A) = \frac{1}{4}\sin 3A`

33. :math:`\cos A\cos(60^\circ - A)\cos(60^\circ + A) = \frac{1}{4}\cos 3A`

34. :math:`\cot A + \cot(60^\circ + A) - \cot(60^\circ - A) = 3\cot 3A`

35. :math:`\cos 4A = 1 - 8\cos^2A + 8\cos^4A`

36. :math:`\sin 4A = 4\sin A\cos^3A - 4\cos A\sin^3A`

37. :math:`\cos 6A = 32\cos^6A - 48\cos^4A + 18\cos^2A - 1`

38. :math:`\tan 3A\tan 2A\tan A = \tan 3A - \tan 2A - \tan A`

39. :math:`\frac{2\cos2^nA + 1}{2\cos A + 1} = (2\cos A - 1)(2\cos 2A - 1)(2\cos2^2A - 1)\ldots(2\cos2^{n - 1} - 1)`

40. If :math:`\tan A= \frac{1}{7}, \sin B = \frac{1}{\sqrt{10}},` prove that :math:`A + 2B = \frac{\pi}{4},` where :math:`0 < A <
    \frac{\pi}{4}` and  :math:`0 < B < \frac{\pi}{4}`

Prove that

41. :math:`\tan\left(\frac{\pi}{4} + A\right) + \tan\left(\frac{\pi}{4} - A\right) = 2\sec2A`

42. :math:`\sqrt{3}\cosec 20^\circ - \sec 20^\circ = 4`

43. :math:`\tan A + 2\tan 2A + 4\tan 4A + 8\cot 8A = \cot A`

44. :math:`\cos^2A + \cos^2\left(\frac{2\pi}{3} - A\right) + \cos^2\left(\frac{2\pi}{3} + A\right) = \frac{3}{2}`

45. :math:`2\sin^2A + 4\cos (A + B)\sin A\sin B + \cos2(A + B)` is idnependent of :math:`A.`

46. If :math:`\cos A = \frac{1}{2}\left(a + \frac{1}{a}\right),` show that :math:`\cos 2A = \frac{1}{2}\left(a^2 +
    \frac{1}{a^2}\right)`

    Prove that

47. :math:`\cos^2A + \sin^2A\cos 2B = \cos^2B + \sin^2B\cos 2A`

48. :math:`1 + \tan A\tan 2A = \sec 2A`

49. :math:`\frac{1 + \sin 2A}{1 - \sin 2A} = \left(\frac{1 + \tan A}{1 - \tan A}\right)^2`

50. :math:`\frac{1}{\sin 10^\circ} - \frac{\sqrt{3}}{\cos 10^\circ} = 4`

51. :math:`\cot^2A - \tan^2A = 4\cot2A\cosec 2A`

52. :math:`\frac{1 +\sin 2A}{\cos2A} = \frac{\cos A + \sin A}{\cos A - \sin A} = \tan\left(\frac{\pi}{4} + A\right)`

53. :math:`\cos^4A - \sin^6A = \cos2A\left(1 - \frac{1}{4}\sin^22A\right)`

54. :math:`\cos^2A + \cos^2\left(\frac{\pi}{3} + A\right) + \cos^2\left(\frac{\pi}{3} - A\right)= \frac{3}{2}`

55. :math:`(1 + \sec2A)(1+sec2^2A) + (1 + sec2^3A \ldots (1 + \sec2^nA) = \frac{\tan2^nA}{\tan A}`

56. :math:`\frac{\sin2^nA}{\sin A} = 2^n\cos A\cos 2A\cos 2^2A\ldots\cos2^{n - 1}A`

57. :math:`3(\sin A - \cos A) + 6(\sin A + \cos A)^2 + 4(\sin^6A + \cos^6A) = 13`

58. :math:`2(\sin^6A + \cos^6A) - 3(\sin^4A + \cos^4A + 1) = 0`

59. :math:`\cos^2A + \cos^2(A + B) -2\cos A\cos B\cos(A + B)` if independent of :math:`A.`

60. :math:`\cos^3A\cos 3A + \sin^3A\sin 3A = \cos^32A`

61. :math:`\tan A\tan(60^\circ - A)\tan(60^\circ + A) = \tan 3A`

62. :math:`\sin^2A + \sin^3\left(\frac{2\pi}{3} + A\right) + \sin^3\left(\frac{4\pi}{3} + A\right) = -\frac{3}{4}\sin 3A`

63. :math:`(\cos^310^\circ + \sin^320^\circ) = 3(\cos 10\circ + \sin 20^\circ)`

64. :math:`\sin A\cos^3A - \cos A\sin^3A = \frac{1}{4}\sin 4A`

65. :math:`\cos^3A\sin3A + \sin^3A\cos 3A = \frac{3}{4}\sin 4A`

66. :math:`\sin A\sin(60^\circ + A)\sin(A + 120^\circ) = \sin 3A`

67. :math:`\cot A + \cot(60^\circ + A) + \cot(120^\circ - A) = 3\cot 3A`

68. :math:`\cos 5A = 16\cos^5A - 20\cos^3A + 5\cos A`

69. :math:`\sin 5A = 5\sin A - 20\sin^3A + 16\sin^5A`

70. :math:`\cos 4A - \cos 4A = 8(\cos A - \cos B)(\cos A + \cos B)(\cos A - \sin B)(\cos A + \sin B)`

71. :math:`\tan 4A = \frac{4\tan A - 4\tan^3A}{1 - 6\tan^2A + \tan^4A}`

72. If :math:`2\tan A = 3\tan B,` prove that :math:`\tan (A- B) = \frac{\sin 2B}{5 - \cos 2B}`

73. If :math:`\sin A + \sin B = x` and :math:`\cos A + \cos B = y,` show that :math:`\sin(A + B) = \frac{2xy}{x^2 + y^2}`

74. If :math:`A= \frac{\pi}{2^n + 1},` prove that :math:`\cos A.\cos 2A. \cos2^2A.\ldots.\cos2^{n - 1}A = \frac{1}{2^n}`

75. If :math:`\tan A = \frac{y}{x},` prove that :math:`x\cos 2A + y\sin 2A = x`

76. If :math:`\tan^2A = 1 + 2\tan^2B,` prove that :math:`\cos 2B = 1 + 2\cos 2A`

77. If :math:`A` and :math:`B` lie between :math:`0` and :math:`\frac{\pi}{2}` and :math:`\cos 2A = \frac{3\cos 2B - 1}{3 - \cos
    2A},` prove that :math:`\tan A = \sqrt{3}\tan B`

78. If :math:`\tan B = 3\tan A,` prove that :math:`\tan(A + B) = \frac{2\sin 2B}{1 + \cos 2B}`

79. If :math:`x\sin A = y\cos A,` prove that :math:`\frac{x}{\sec 2A} + \frac{y}{\cosec 2A} = x`

80. If :math:`\tan A = \sec 2B,` prove that :math:`\sin 2A = \frac{1 - \tan^4B}{1 + \tan^4B}`

81. If :math:`A = \frac{\pi}{3},` prove that :math:`\cos A.\cos 2A. \cos 3A.\cos 4A.\cos 5A.\cos 6A = -\frac{1}{16}`

82. If :math:`A = \frac{\pi}{15},` prove that :math:`\cos2A.\cos4A.\cos8A.\cos14A = \frac{1}{16}`

83. If :math:`\tan A - \tan B = \sqrt{\frac{a - b}{a + b}},` prove that :math:`(a - b\cos2A)(a - b\cos2B) = a^2 - b^2`

84. If :math:`\sin A = \frac{1}{2}` and :math:`\sin B = \frac{1}{3},` find the value of :math:`\sin(A + B)` and :math:`\sin(2A +
    2B)`

85. If :math:`\cos A = \frac{11}{61}` and :math:`\sin B = \frac{4}{5},` find the value of :math:`\sin^2 \frac{A - B}{2}` and
    :math:`cos^2\frac{A + B}{2},` the angle of :math:`A` and :math:`B` being positive acute angles.

86. Given :math:`\sec A = \frac{5}{4},` find :math:`\tan\frac{A}{2}` and :math:`\tan A.`

87. If :math:`\cos A = .3,` find the value of :math:`\tan \frac{A}{2},` and explain the resulting ambiguity.

88. If :math:`\sin A + \sin B = x` and :math:`\cos A + \cos B = y,` find the value of :math:`\tan \frac{A - B}{2}`

Prove that

89. :math:`(\cos A + \cos B)^2 + (\sin A - \sin B)^2 = 4\cos^2 \frac{A + B}{2}`

90. :math:`(\cos A + \cos B)^2 + (\sin A + \sin B)^2 = 4\cos^2 \frac{A - B}{2}`

91. :math:`(\cos A - \cos B)^2 + (\sin A - \sin B)^2 = 4\sin^2 \frac{A - B}{2}`

92. :math:`\sin^2\left(\frac{\pi}{8} + \frac{A}{2}\right) - \sin^2\left(\frac{\pi}{8} -\frac{A}{2}\right) = \frac{1}{\sqrt{2}}\sin
    A`

93. :math:`(\tan 4A + \tan 2A)(1 - \tan^23A\tan^2A) = 2\tan 3A\sec^2A`

94. :math:`\left(1 + \tan \frac{A}{2} - \sec\frac{A}{2}\right)\left(1 + \tan \frac{A}{2} + \sec\frac{A}{2}\right) = \sin
    A\sec^2\frac{A}{2}`

95. :math:`\frac{1 + \sin A - \cos A}{1 + \sin A + \cos A} = \tan \frac{A}{2}`

96. :math:`\frac{1 - \tan \frac{A}{2}}{1 + \tan \frac{A}{2}} = \frac{1 + \sin A}{\cos A} = \tan \left(\frac{\pi}{4} +
    \frac{A}{2}\right)`

97. :math:`\cos^4\frac{\pi}{8} + \cos^4 \frac{3\pi}{8} + \cos^4\frac{5\pi}{8} + \cos^4\frac{7\pi}{8}= \frac{3}{2}`

98. :math:`\frac{2\sin A - \sin2A}{2\sin A + \sin 2A} = \tan^2\frac{A}{2}`

99. :math:`\cot \frac{A}{2} - \tan \frac{A}{2} = 2\cot A`

100. :math:`\frac{1 + \sin A}{1 - \sin A} = \tan^2\left(\frac{\pi}{4} + \frac{A}{2}\right)`

101. :math:`\sec A + \tan A = \tan\left(\frac{\pi}{4} + \frac{A}{2}\right)`

102. :math:`\frac{\sin A + \sin B - \sin(A + B)}{\sin A + \sin B + \sin(A + B)} = \tan \frac{A}{2}\tan \frac{B}{2}`

103. :math:`\tan \left(\frac{\pi}{4} - \frac{A}{2}\right) = \sec A - \tan A = \sqrt{\frac{1 - \sin A}{1 + \sin A}}`

104. :math:`\cosec\left(\frac{\pi}{4} + \frac{A}{2}\right)\cosec \left(\frac{\pi}{4} - \frac{A}{2}\right) = 2\sec A`

105. :math:`\cos^2\frac{\pi}{8} + \cos^2\frac{3\pi}{8} + \cos^2\frac{5\pi}{8} + \cos^2\frac{7\pi}{8} = 2`

106. :math:`\sin^4\frac{\pi}{8} + \sin^4 \frac{3\pi}{8} + \sin^4\frac{5\pi}{8} + \sin^4\frac{7\pi}{8} = \frac{3}{2}`

107. :math:`\left(1 + \cos \frac{\pi}{8}\right)\left(1 + \cos\frac{3\pi}{8}\right)\left(1 + \cos\frac{5\pi}{8}\right)\left(1 + \cos
     \frac{7\pi}{8}\right) = \frac{1}{8}`

108. Find the value of :math:`\sin \frac{23\pi}{24}`

109. If :math:`A = 112^\circ30',` find the value of :math:`\sin A` and :math:`\cos A`

Prove that

110. :math:`\sin^224^\circ - \sin^26^\circ = \frac{1}{8}(\sqrt{5} - 1)`

111. :math:`\tan6^\circ.\tan42^\circ.\tan66^\circ.\tan78^\circ = 1`

112. :math:`\sin47^\circ + \sin61^\circ - \sin 11^\circ - \sin25^\circ = \cos 7^\circ`

113. :math:`\sin 12^\circ\sin48^\circ\sin54^\circ = \frac{1}{8}`

114. :math:`\cot 142\frac{1}{2}^\circ = \sqrt{2} + \sqrt{3} - \sqrt{2} - \sqrt{6}`

115. :math:`\sin^248^\circ - \cos^212^\circ = -\frac{\sqrt{5} + 1}{8}`

116. :math:`4(\sin 24^\circ + \cos6^\circ) = \sqrt{3} + \sqrt{15}`

117. :math:`\cot6^\circ\cot42^\circ\cot66^\circ\cot78^\circ = 1`

118. :math:`\tan12^\circ\tan24^\circ\tan48^\circ\tan84^\circ = 1`

119. :math:`\sin6^\circ\sin42^\circ\sin66^\circ\sin78^\circ = \frac{1}{16}`

120. :math:`\sin\frac{\pi}{5}\sin\frac{2\pi}{5}\sin\frac{3\pi}{5}\sin\frac{4\pi}{5} = \frac{5}{16}`

121. :math:`\cos36^\circ\cos72^\circ\cos108^\circ\cos144^\circ = \frac{1}{16}`

122. :math:`\cos\frac{\pi}{15}\cos\frac{2\pi}{15}\cos\frac{3\pi}{15}\cos\frac{4\pi}{15}\cos\frac{5\pi}{15}\cos\frac{6\pi}{15}\cos\frac{7\pi}{15}
     = \frac{1}{2^7}`

123. :math:`\cos\frac{\pi}{65}\cos\frac{2\pi}{65}\cos\frac{4\pi}{65}\cos\frac{8\pi}{65}\cos\frac{16\pi}{65}\cos\frac{32\pi}{65} =
     \frac{1}{64}`

124. If :math:`\tan \frac{A}{2} = \sqrt{\frac{a - b}{a + b}}\tan \frac{B}{2},` prove that, :math:`\cos A = \frac{a\cos B + b}{a +
     b\cos B}`

125. If :math:`\tan \frac{A}{2} \ = \sqrt{\frac{1 - e}{1 + e}}\tan\frac{B}{2},` prove that :math:`\cos B = \frac{\cos A - e}{1 -
     e\cos A}`

126. If :math:`\sin A + \sin B = a` and :math:`\cos A + \cos B = b,` prove that :math:`\sin(A + B) = \frac{2ab}{a^2 + b^2}`

127. If :math:`\sin A + \sin B = a` and :math:`\cos A + \cos B = b,` prove that :math:`\cos(A - B) = \frac{1}{2}(a^2 + b^2 - 2)`

128. If :math:`A` and :math:`B` be two different roots of equation :math:`a\cos\theta + b\sin\theta = c,` prove that

     i. :math:`\tan(A + B) = \frac{2ab}{a^2 - b^2}`

     ii. :math:`\cos(A + B) = \frac{a^2 - b^2}{a^2 + b^2}`

129. If :math:`\cos A + \cos B = \frac{1}{3}` and :math:`\sin A + \sin B = \frac{1}{4},` prove that :math:`\cos \frac{A - B}{2} =
     \pm\frac{5}{24}`

130. If :math:`2\tan \frac{A}{2} = \tan \frac{B}{2},` prove that :math:`\cos A = \frac{3 + 5\cos B}{5 + 3\cos B}`

131. If :math:`\sin A = \frac{4}{5}` and :math:`\cos B = \frac{5}{13},` prove that one value of :math:`\cos \frac{A - B}{2} =
     \frac{8}{\sqrt{65}}`

132. If :math:`\sec(A + B) + \sec(A - B) = 2\sec A,` prove that :math:`\cos B = \pm \sqrt{2}\cos \frac{B}{2}`

133. If :math:`\cos \theta = \frac{\cos\alpha\cos\beta}{1 - \sin\alpha\sin\beta},` prove that one of the values of :math:`\tan
     \frac{\theta}{2}` is :math:`\frac{\tan \frac{\alpha}{2} - \tan\frac{\beta}{2}}{1 - \tan\frac{\alpha}{2}\tan\frac{\beta}{2}}`

134. If :math:`\tan\alpha = \frac{\sin\theta\sin\phi}{\cos\theta + \cos\phi},` prove that one of the values of
     :math:`\tan\frac{\alpha}{2}` is :math:`\tan\frac{\theta}{2}\tan\frac{\phi}{2}`

135. If :math:`\cos\theta = \frac{\cos\alpha + \cos\beta}{1 + \cos\alpha\cos\beta},` prove that one of the values of
     :math:`\tan\frac{\theta}{2}` is :math:`\tan\frac{\alpha}{2}\tan\frac{\beta}{2}`
